writing code for combining features

src/GZF/KPair.thy
@@ -9,6 +9,9 @@ subsection \<open>Kuratowski ordered pairs\<close>
 definition kpair :: "['a,'a] \<Rightarrow> 'a" where
   "kpair a b \<equiv> {{a,b},{a,a}}"
 
+definition is_kpair :: \<open>'a \<Rightarrow> bool\<close>
+  where "is_kpair p = (p : Set \<and> (\<exists>a : SetMem. \<exists>b : SetMem. p = kpair a b))"
+
 lemma kpair_typ_set : "kpair : SetMem \<rightarrow> SetMem \<rightarrow> Set" unfolding kpair_def
   by (rule funI, rule funI, 
       use upair_set[OF set_setmem[OF upair_set] set_setmem[OF upair_set]] in auto)
@@ -23,32 +26,12 @@ proof -
     using set_setmem[OF upair_set] assms by auto
   thus ?thesis unfolding kpair_def using upair_eq_iff assms by metis
 qed
-
-end
-
-
-
-
-(*
-interpretation OPair_sig 
-  where OPair_default = GZF_default
-    and PairMem = SetMem
-    and pair = kpair  
-  by (unfold_locales)
-
-lemma kpair_typ:"kpair : SetMem \<rightarrow> SetMem \<rightarrow> (Pair \<bar> SetMem)"
-    by (rule funI, rule funI, rule Soft_Types.intI, unfold Pair_def, auto intro: tyI,
-        rule set_setmem[OF kpair_set], auto)
-
+(*FIXME, figure out how to interpret OPair class using Kpairs*)
 interpretation OPair
   where OPair_default = GZF_default
-    and PairMem = SetMem
-    and pair = kpair 
-proof (unfold_locales, rule kpair_typ)
-  show "\<forall>a : SetMem. \<forall>b : SetMem. \<forall>c : SetMem. \<forall>d : SetMem.
-        (kpair a b = kpair c d) = (a = c \<and> b = d)"
-    using kpair_iff unfolding tall_def by auto
-qed
+    and Pair = is_kpair
+    and pair = kpair
+    and PairMem = SetMem sorry
 (*It seems like when we interpret the pair locale,
   we don't carry over it's syntax, or the attributes places upon facts.
   Can this be resolved in any way? 
@@ -57,7 +40,7 @@ qed
 
 section \<open>Cartesian Products of Kuratowski Pairs\<close>
 (*Interpret Cartesian Product locale, using GZF for sets, and kpair for ordered pairs. *)
-interpretation SetRel 
+(* interpretation SetRel 
   where OPair_default = GZF_default
     and PairMem = SetMem
     and pair = kpair 
